Primitive_TMs.thy
@@ -30,4 +30,85 @@ proof (intro valid_TM_I)
   with \<open>length hds = k\<close> and \<open>set hds \<subseteq> options \<Sigma>\<close> show "hds ! i \<in> options \<Sigma>" by fastforce
 qed (use assms in blast)+
 
+
+definition "read_TM_M k \<Sigma> \<equiv> Abs_TM (read_TM_rec k \<Sigma>)"
+
+locale read_TM = TM "Abs_TM (read_TM_rec k \<Sigma>)"
+  for k :: nat and \<Sigma> :: "'s set" +
+  assumes at_least_one_tape: "k > 0"
+    and finite_symbols: "finite \<Sigma>"
+    and nonempty_symbols: "\<Sigma> \<noteq> {}"
+begin
+
+lemma M_rec: "M_rec = read_TM_rec k \<Sigma>" using read_TM_rec_valid[OF at_least_one_tape finite_symbols nonempty_symbols]
+  by (intro Abs_TM_inverse CollectI)
+
+lemma M_fields:
+  shows "tape_count \<equiv> k"
+    and "symbols \<equiv> \<Sigma>"
+    and "Q \<equiv> options (options \<Sigma>)"
+    and "q\<^sub>0 \<equiv> None"
+    and "F \<equiv> Some ` options \<Sigma>"
+    and "label \<equiv> the"
+    and "\<delta>\<^sub>q \<equiv> \<lambda>q hds. Some (hd hds)"
+    and "\<delta>\<^sub>w \<equiv> \<lambda>q. (!)"
+    and "\<delta>\<^sub>m \<equiv> \<lambda>q hds i. No_Shift"
+  unfolding TM_fields_defs M_rec unfolding read_TM_rec_def TM_record.simps .
+
+declare M_fields(1-6)[simp]
+
+
+lemma step:
+  assumes "state c = q\<^sub>0"
+    and "wf_config c"
+  shows "step c = TM_config (Some (head (hd (tapes c)))) (tapes c)"
+  using assms
+proof (induction c)
+  case (TM_config q tps)
+  let ?c = "TM_config q tps"
+  let ?h = "head (hd tps)"
+
+  assume "state ?c = q\<^sub>0"
+  then have [simp]: "q = q\<^sub>0" by simp
+  assume "wf_config ?c"
+  from wf_configD(2)[OF this] have [simp]: "length tps = tape_count" by simp
+  from \<open>wf_config ?c\<close> have "tps \<noteq> []" by force
+
+  have "step ?c = step_not_final ?c" by force
+  also have "... = TM_config (Some ?h) tps"
+  proof (rule TM_config_eq, unfold step_not_final_simps TM_config.sel)
+    show "\<delta>\<^sub>q q (map head tps) = Some ?h" unfolding M_fields list.map_sel[OF \<open>tps \<noteq> []\<close>] ..
+
+    show "map2 tape_action (\<delta>\<^sub>a q (map head tps)) tps = tps"
+    proof (rule step_not_final_eqI)
+      fix i
+      assume "i < tape_count"
+      then have "i < length tps" by simp
+      then show "tape_action (\<delta>\<^sub>w q (map head tps) i, \<delta>\<^sub>m q (map head tps) i) (tps ! i) = tps ! i"
+        unfolding M_fields by simp
+    qed auto
+  qed
+  also have "... = TM_config (Some (head (hd (tapes ?c)))) (tapes ?c)" by simp
+  finally show ?case .
+qed
+
+
+lemma
+  assumes "state c = q\<^sub>0"
+    and "wf_config c"
+  shows "is_final (step c)"
+    and "conf_label (step c) = head (hd (tapes c))"
+    and "tapes (step c) = tapes c"
+proof -
+  show [simp]: "tapes (step c) = tapes c" unfolding step[OF assms] by simp
+  have [simp]: "state (step c) = Some (head (hd (tapes c)))" unfolding step[OF assms] by simp
+
+  from \<open>wf_config c\<close> have "head (hd (tapes c)) \<in> \<Sigma>\<^sub>t\<^sub>p" by fastforce
+  then show "is_final (step c)" unfolding is_final_def by simp
+
+  show "conf_label (step c) = head (hd (tapes c))" by simp
+qed
+
+end \<comment> \<open>\<^locale>\<open>read_TM\<close>\<close>
+
 end
